Fix .proj case

tests/projects/disproof_structural_rigidity_mismatch/Challenge.lean
@@ -1,6 +1,6 @@
 /- Tests static type and universe level inference for structure projections on fields with varying universe levels. -/
 structure MyStruct.{u} where
   A : Type u
-  B : Prop
+  B : Type u
 
 theorem foo (s : MyStruct.{1}) (h : s.B) : False := sorry
